backends/lean/Aeneas/SLPoC/Tests/Examples/IrisTutorial.lean
@@ -1,4 +1,4 @@
-import Aeneas.SLPoC.Step
+import Aeneas.SLPoC.RustHeap
 
 namespace Aeneas.SLPoC
 
